proof/contract/lemmas.v
@@ -13,3 +13,4 @@ From wots Require Export contract.lemmas.chain.
 From wots Require Export contract.lemmas.arith.
 From wots Require Export contract.lemmas.pkgen_sign.
 From wots Require Export contract.lemmas.verify.
+From wots Require Export contract.lemmas.null_check.
